pulse/lib/steel/pulse/Pulse.Checker.Bind.fsti
@@ -9,6 +9,8 @@ open Pulse.Elaborate.Pure
 open Pulse.Typing
 open Pulse.Checker.Common
 
+let st_comp_with_pre (st:st_comp) (pre:term) : st_comp = { st with pre }
+
 val mk_bind (g:env)
             (pre:term)
             (e1:st_term)
@@ -22,7 +24,7 @@ val mk_bind (g:env)
             (res_typing:universe_of g (comp_res c2) (comp_u c2))
             (post_typing:tot_typing (extend (snd px) (Inl (comp_res c2)) g) (open_term_nv (comp_post c2) px) Tm_VProp)
   : T.TacH (t:st_term &
-            c:comp { stateful_comp c ==> comp_pre c == pre } &
+            c:comp_st { st_comp_of_comp c == st_comp_with_pre (st_comp_of_comp c2) pre } &
             st_typing g t c)
            (requires fun _ ->
               let _, x = px in
@@ -35,7 +37,7 @@ val mk_bind (g:env)
 
 val bind_res_and_post_typing (g:env) (s2:st_comp)
                              (x:var { Pulse.Typing.Metatheory.fresh_wrt x g (freevars s2.post) })
-                             (post_hint:post_hint_opt g)
+                             (post_hint:post_hint_opt g { comp_post_matches_hint (C_ST s2) post_hint })
   : T.Tac (universe_of g s2.res s2.u &
            tot_typing (extend x (Inl s2.res) g) (open_term_nv s2.post (v_as_nv x)) Tm_VProp)
 
@@ -45,9 +47,7 @@ val check_bind (g:env)
                (pre_typing:tot_typing g pre Tm_VProp)
                (post_hint:post_hint_opt g)               
                (check:check_t)
-  : T.Tac (t:st_term &
-           c:comp { stateful_comp c ==> comp_pre c == pre } &
-           st_typing g t c)
+  : T.Tac (checker_result_t g pre post_hint)
 
 val check_tot_bind
   (g:env)
@@ -56,7 +56,4 @@ val check_tot_bind
   (pre_typing:tot_typing g pre Tm_VProp)
   (post_hint:post_hint_opt g)
   (check:check_t)
-  : T.Tac (t:st_term &
-           c:comp { stateful_comp c ==> comp_pre c == pre } &
-           st_typing g t c)
-
+  : T.Tac (checker_result_t g pre post_hint)
