pulse/lib/steel/pulse/Pulse.Checker.Common.fsti
@@ -103,32 +103,17 @@ val try_frame_pre (#g:env)
   : T.Tac (c':comp_st { comp_pre c' == pre } &
            st_typing g t c')
 
-val replace_equiv_post
-      (g:env)
-      (c:comp{stateful_comp c /\ freevars_comp c `Set.subset` FV.vars_of_env g})
-      (ct:Metatheory.comp_typing_u g c)
-      (post_hint:post_hint_opt g)
-  : T.Tac (c1:comp { stateful_comp c1 /\ comp_pre c1 == comp_pre c } & st_equiv g c c1)
-
-val repack (#g:env) (#pre:term) (#t:st_term)
-           (x:(c:comp_st { comp_pre c == pre } & st_typing g t c))
-           (post_hint:post_hint_opt g)
-           (apply_post_hint:bool)
-  : T.Tac (t:st_term &
-           c:comp {stateful_comp c ==> comp_pre c == pre} &
-           st_typing g t c)
-
-val intro_comp_typing (g:env) 
-                      (c:comp_st)
-                      (pre_typing:tot_typing g (comp_pre c) Tm_VProp)
-                      (res_typing:universe_of g (comp_res c) (comp_u c))
-                      (x:var { Metatheory.fresh_wrt x g (freevars (comp_post c)) })
-                      (post_typing:tot_typing (extend x (Inl (comp_res c)) g) (open_term (comp_post c) x) Tm_VProp)
-  : T.Tac (comp_typing g c (comp_u c))
+let comp_post_matches_hint (c:comp_st) (post_hint:option post_hint_t) =
+  match post_hint with
+  | None -> True
+  | Some post_hint ->
+    comp_res c == post_hint.ret_ty /\
+    comp_u c == post_hint.u /\
+    comp_post c == post_hint.post
 
 let checker_result_t (g:env) (pre:term) (post_hint:option post_hint_t) =
     t:st_term &
-    c:comp{stateful_comp c ==> comp_pre c == pre} &
+    c:comp{stateful_comp c ==> comp_pre c == pre /\ comp_post_matches_hint c post_hint } &
     st_typing g t c
 
 let continuation_elaborator (g:env) (ctxt:term)
@@ -144,3 +129,16 @@ type check_t =
   pre_typing:tot_typing g pre Tm_VProp ->
   post_hint:post_hint_opt g ->
   T.Tac (checker_result_t g pre post_hint)
+
+val repack (#g:env) (#pre:term) (#t:st_term)
+           (x:(c:comp_st { comp_pre c == pre } & st_typing g t c))
+           (post_hint:post_hint_opt g)
+  : T.Tac (checker_result_t g pre post_hint)
+
+val intro_comp_typing (g:env) 
+                      (c:comp_st)
+                      (pre_typing:tot_typing g (comp_pre c) Tm_VProp)
+                      (res_typing:universe_of g (comp_res c) (comp_u c))
+                      (x:var { Metatheory.fresh_wrt x g (freevars (comp_post c)) })
+                      (post_typing:tot_typing (extend x (Inl (comp_res c)) g) (open_term (comp_post c) x) Tm_VProp)
+  : T.Tac (comp_typing g c (comp_u c))
