pulse/lib/steel/pulse/Pulse.Checker.Exists.fsti
@@ -12,9 +12,7 @@ val check_elim_exists
   (pre:term)
   (pre_typing:tot_typing g pre Tm_VProp)
   (post_hint:post_hint_opt g)
-  : T.Tac (t:st_term &
-           c:comp{stateful_comp c ==> comp_pre c == pre} &
-           st_typing g t c)
+  : T.Tac (checker_result_t g pre post_hint)
 
 let intro_exists_witness_singleton (st:st_term)  = 
   match st.term with
@@ -32,6 +30,4 @@ val check_intro_exists_either
   (pre:term)
   (pre_typing:tot_typing g pre Tm_VProp)
   (post_hint:post_hint_opt g)
-  : T.Tac (t:st_term &
-           c:comp{stateful_comp c ==> comp_pre c == pre} &
-           st_typing g t c)
+  : T.Tac (checker_result_t g pre post_hint)
