pulse/lib/steel/pulse/Pulse.Checker.Framing.fst
@@ -225,6 +225,7 @@ let apply_frame (#g:env)
                 (frame_t:frame_for_req_in_ctxt g ctxt (comp_pre c))
   : Tot (c':comp_st { comp_pre c' == ctxt /\
                       comp_res c' == comp_res c /\
+                      comp_u c' == comp_u c /\
                       comp_post c' == Tm_Star (comp_post c) (frame_of frame_t) } &
            st_typing g t c')
   = let s = st_comp_of_comp c in
