pulse/lib/steel/pulse/Pulse.Checker.If.fst
@@ -21,7 +21,7 @@ let rec combine_if_branches
   (e_else:st_term)
   (c_else:comp_st)
   (e_else_typing:st_typing g_else e_else c_else)
-  : T.TacH (c:comp_st{comp_pre c == comp_pre c_then} &
+  : T.TacH (c:comp_st{st_comp_of_comp c == st_comp_of_comp c_then} &
             st_typing g_then e_then c &
             st_typing g_else e_else c)
            (requires fun _ ->
@@ -72,6 +72,7 @@ let rec combine_if_branches
   else T.fail "Cannot combine then and else branches (different st_comp)"
 #pop-options
 
+#push-options "--query_stats --ifuel 2 --z3rlimit_factor 4"
 let check_if (g:env)
              (b:term)
              (e1 e2:st_term)
@@ -79,9 +80,7 @@ let check_if (g:env)
              (pre_typing: tot_typing g pre Tm_VProp)
              (post_hint:post_hint_for_env g)
              (check:check_t)
-  : T.Tac (t:st_term &
-           c:comp { stateful_comp c ==> comp_pre c == pre } &
-           st_typing g t c)
+  : T.Tac (checker_result_t g pre (Some post_hint))
   = let (| b, b_typing |) =
       check_term_with_expected_type g b tm_bool in
     let post = post_hint.post in
@@ -91,7 +90,7 @@ let check_if (g:env)
     in
     let check_branch (eq_v:term) (br:st_term)
       : T.Tac (br:st_term { ~(hyp `Set.mem` freevars_st br) } &
-               c:comp { stateful_comp c /\ comp_pre c == pre } &
+               c:comp { stateful_comp c /\ comp_pre c == pre /\ comp_post_matches_hint c (Some post_hint)} &
                st_typing (g_with_eq eq_v) br c)
       = let g_with_eq = g_with_eq eq_v in
         let pre_typing = 
@@ -104,10 +103,10 @@ let check_if (g:env)
         in
         if hyp `Set.mem` freevars_st br
         then T.fail "Illegal use of control-flow hypothesis in branch"
-        else if C_Tot? c
+        else if not (stateful_comp c)
         then T.fail "Branch computation type not st"
         else (| br, c, br_typing |)
-    in
+    in 
     let (| e1, c1, e1_typing |) = check_branch tm_true e1 in
     let (| e2, c2, e2_typing |) = check_branch tm_false e2 in    
     let (| c, e1_typing, e2_typing |) =
