pulse/lib/steel/pulse/Pulse.Checker.WithLocal.fsti
@@ -14,6 +14,4 @@ val check_withlocal
   (pre_typing:tot_typing g pre Tm_VProp)
   (post_hint:post_hint_opt g)
   (check':bool -> check_t)
-  : T.Tac (t:st_term &
-           c:comp{stateful_comp c ==> comp_pre c == pre} &
-           st_typing g t c)
+  : T.Tac (checker_result_t g pre post_hint)
